engine/PrisonersDilemma.lean
@@ -2,8 +2,13 @@
 -- Import modules here that should be built as part of the library.
 import PrisonersDilemma.Core
 import PrisonersDilemma.Pipeline
-import PrisonersDilemma.Models.Simple
+import PrisonersDilemma.StrategyDSL
+import PrisonersDilemma.Models.CooperateBot
+import PrisonersDilemma.Models.DefectBot
+import PrisonersDilemma.Models.DBotIsolated
 import PrisonersDilemma.Models.OpenSourceBots
-import PrisonersDilemma.Proofs.Simple
 import PrisonersDilemma.Proofs.WorkflowTemplate
+import PrisonersDilemma.Proofs.CooperateBot
+import PrisonersDilemma.Proofs.DefectBot
+import PrisonersDilemma.Proofs.DBotIsolated
 import PrisonersDilemma.Proofs.OpenSourceBots
